tags: #notes #fleeting  
creation date: [[2022-11-11 Friday]] 11:31:52  
description:: structural induction

I didn't take notes it's 11:32 oops I was just looking at my phone not paying attention

So far he's talked about uhh  
  
Binary tree  
Some new kind of induction or something

Proof by induction ab binary tree



Nov. 16: writing these notes now bc i need them for hw 9

Structural induction is used to prove properties of recursive structures. To prove a property S(X) of a recursively defined structure X, it is sufficient to prove that S(X) is true for the basis structures of X and that $S(Y_1) \wedge S(Y_2) \wedge \ldots \wedge S(Y_k) \rightarrow S(X)$, where X is constructed from $Y_1, Y_2, \ldots, Y_k$.

ex. Let the height of a tree be the number of nodes on the longest path from the root to a leaf (note that height of $\emptyset$ is 0). Prove that for any binary tree with $n$ nodes and height $h$, $n \leq 2^h - 1$.

##### Proof by inducting on height
Basis step: consider the empty tree. obviously $n = 0$ and $h = 0$ which satisfies the inequality

I.H.: assume for any binary tree with height up to $k$, the inequality holds

I.S.: consider binary tree with height $k + 1$
![[Pasted image 20221116201147.png]]
assume that the left subtree has $n_1$ nodes with height $h_1$ an and the right subtree has $n_2$ nodes with height $h_2$. thus $k + 1 = max(h_1, h_2) + 1$

since $h_1, h_2 \leq k$, then by IH, $n_1 \leq 2^{h_1} - 1$ and $n_2 \leq 2^{h_2} - 1$
so $n = n_1 + n_2 + 1$
$\leq ( 2^{h_1} - 1) + ( 2^{h_2} - 1) + 1$
$\leq 2^{max(h_1, h_2) + 1} - 1 = 2^{k+1} - 1$


##### Structural induction proof
yeah that wasn't even the structural induction proof ok

Basis step: consider the empty tree. obviously $n = 0$ and $h = 0$ which satisfies the inequality

I.H.: Assume for two binary trees $T_1$ and $T_2$ the inequality holds.

I.S.: We will prove that the inequality holds also for the tree built recursively from these two trees. This tree is built as a new root with $T_1$ and $T_2$ as its left and right subtrees.

Assume that $T_1$ has $n_1$ nodes with height $h_1$ and $T_2$ has $n_2$ nodes with height $h_2$. Thus the hight of the new tree is $h = max(h_1, h_2) + 1$

By IH, $n_1 \leq 2^{h_1} - 1$ and $n_2 \leq 2^{h_2} - 1$.
So $n = n_1 + n_2 + 1$
$\leq ( 2^{h_1} - 1) + ( 2^{h_2} - 1) + 1$
$\leq 2^{max(h_1, h_2) + 1} - 1 = 2^{k+1} - 1$


Notice the two proofs are almost identical
Structural induction simply removes the need to induct on a particular variable, instead using the recursive definition as the step between I.H. and I.S.