tags: #notes #fleeting
creation date: [[2022-10-10 Monday]] 10:57:11
description:: even more sums

test
m,an pls get closer to the mic what is he saying
open note
summations will be on it
"waste tyime searching through the notes" ahahaha i have obsidian search

##### Factoring out
![[Pasted image 20221010110829.png]]
factors that do not depend on the summation index can be factored out
![[Pasted image 20221010110904.png]]

$\sum^n_{i=1} \sum^n_{j=1} a_i b_j = \sum^n_{i=1} a_i \sum^n_{j=1} b_j$
also can switch the above
$\sum^n_{i=1} a_i \sum^n_{j=1} b_j = \sum^n_{j=1} b_j \sum^n_{i=1} a_i$


##### Double summation
a sequence could have two (or more) indices
$a_{ij}$

ex. $a_{ij} = (3i)^j$
can represent as a 2D matrix
![[Pasted image 20221010111337.png]]

double summation is like two nested for loops

![[Pasted image 20221010112036.png]]
can sum over these loops either way


##### Some useful summations
- Arithmetic series
- Geometric series
- Sum of squares
	- $\sum^n_{j=1} j^2 = 1^2 + 2^2 + 3^2 + ... + n^2$
	- $= \frac 1 6 n (n+1) (2n+1)$
	- would need to prove something like this by induction on the test ? is that what he said
	- also need to prove on the hw
	- ummm ok
- Sum of cubes
	- $\sum^n_{j=1} j^3 = 1^3 + 2^3 + 3^3 + ... + n^3$
	- $= \frac 1 4 n^2 (n+1)^2$
- Proof of squares
	- Let $S = \sum^n_{j=1} j^2$
	- First lets replace $j^2$ with an arithmetic summation
		- Let $a, d$ be the parameters of the arithmetic series
		- Then $\sum^n_{j=1} (a + id) = aj + d \frac {j(j+1)} {2} = j^2$
		- Choosing $d = 2$ gives $a = -1$, and this $\sum^n_{j=1} (2i = 1) = j^2$
	- Thus
		- man i am not writing this out \
		- $S = \sum^n_{j=1} j^2$
		- $= \sum^n_{j=1} \sum^j_{i=1} (2i-1)$
		- $\overset{*}{=}  \sum^n_{j=1} (2j - 1) (n - j + 1)$
			- the asterisk means something idk
		- $= \sum^n_{j=1} (2jn - 2j^2 + 2j - n + j - 1)$
		- $= -2S + \sum^n_{j=1} (2jn + 3j) - n(n+1)$
		- $= -2S + (2n + 3)n(n+1) \frac 1 2 - n(n+1) = S$
		- $\rightarrow 3S = n\frac {(n+1)(2n+1)} 2$
	- what does $\overset{*}{=}$ mean
		- $\sum^n_{j=1} \sum^j_{i=1} (2i-1)$
		- make a table ![[Pasted image 20221010114514.png]]
		- $\sum^n_{j=1} \sum^j_{i=1} (2i-1) \overset{*}{=}  \sum^n_{j=1} (2j - 1) (n - j + 1)$
		- "want you to practice this" man practice what what is this
		- 