tags: #notes #fleeting
creation date: [[2022-09-09 Friday]] 11:02:51
description:: logical laws, predicates, quantifiers

from last class
- number of possible operators: with n variables, $2^{2^n}$ functions


## Laws
##### Identity
- $p \bigwedge T \equiv p$
- $p \bigvee F \equiv p$
leaves p the same

##### Domination
- $p \bigvee T \equiv T$
- $p \bigwedge F \equiv F$
p does not matter

##### Idempotent
- $p \bigvee p \equiv p$
- $p \bigwedge p \equiv p$

##### Double negation
- $\neg (\neg p ) \equiv p$

##### Negation
- $p \bigvee \neg p \equiv T$
- $p \bigwedge  \neg p \equiv F$

##### Absorption
- $p \bigvee (p \bigwedge p) \equiv p$
- $p \bigwedge (p \bigvee p) \equiv p$

"why is absorption law necessary?"
"it is not"
none of these are necessary
we need these to build complex structures easier
- ok so they are necessary we're gonna use them later
"not necessary just making our lives easier"
ok fine
**"gonna use these so we dont have to use truth tables"**

##### Commutative
- $p \bigvee q \equiv q \bigvee p$
- $p \bigwedge q \equiv q \bigwedge p$

"who has taken linear algebra? you know matrix multiplication isnt commutative"
ok spoilers

##### Associative
- $(p \bigvee q) \bigvee r \equiv p \bigvee (q \bigvee r)$
- $(p \bigwedge q) \bigwedge r \equiv p \bigwedge (q \bigwedge r)$

##### Distributive
- $p \bigvee (q \bigwedge r) \equiv (p \bigvee q) \bigwedge (p \bigvee r)$
- $p \bigwedge (q \bigvee r) \equiv (p \bigwedge q) \bigvee (p \bigwedge r)$

"our bread and olive oil"
"do i have to remember the names? no youre not tested on it but you should see these and be able to use them theyll be helpful"

##### De Morgan's Law
- $\neg(p \bigvee q) \equiv \neg p \bigwedge \neg q$
- $\neg(p \bigwedge q) \equiv \neg p \bigvee \neg q$

ex. It is not true that I am old and rich $\equiv$ I am not old or not rich
ex. It is not true that I am old or that I am rich $\equiv$ I am not old and not rich

we can also use this for implication, unlike the other laws
this is useful because we can take an implication and turn it into a form that uses ands and ors, so we can use the other laws

from last class "the breakfast box"
- $p \rightarrow q \equiv \neg p \bigvee q$
add a neg on each side
- $\neg (p \rightarrow q) \equiv \neg (\neg p \bigvee q)$
use de morgan's law
- $\equiv \neg(\neg p ) \bigwedge \neg q$ 
use double negation
- $\equiv p \bigwedge \neg q$

"we have reached the situation where we can get rid of truth tables"


## Predicates
a function P(x) = "x > 3"
P(x) is a proposition of any value of x
ex. P(1) is a proposition, because 1 > 3 is a proposition (a false one)

A **predicate** is a statement with variables. It is either true or false depending on the values assigned to the variables.

typically use Uppercase for predicates
P(x) is a predicate, p is a proposition

another ex. Q(x, y) = "$x^2 + y^2 = 4$"
dont need the quotation marks
typically defined with the notation
let Q(x,y) be the predicate $x^2 + y^2 = 4$

operators can be defined for predicates

P(x) = $x > 1$
Q(x) = $x^3$ is negative

$P(x) \bigwedge Q(x)$
this is always False for all x

$P(x) \rightarrow Q(x)$
Say x = -1
What does this evaluate to?
P(x) is False
Q(x) is True
$F \rightarrow T \equiv T$
so,
$P(-1) \rightarrow Q(-1) \equiv T$

$(x < 0 ) \bigwedge (y > 0) \rightarrow (x * y < 0)$
"if x is negative and y is positive, then their product is negative"
you can pick x and y that dont satisfy this hypothesis, but if the hypothesis of an implication is false, then the implication is true!
(source the truth table $p \rightarrow q$ is always T is p is F)

humans dont think in this logic, they think with statistical logic, based off experience

## Quantifiers
##### Universal
- ∀ for all
- ∀xP(x)
- latex is "forall"

##### Existential
- ∃ there exists
- ∃x(x >3)
- latex is "exists"

##### De Morgan's Law with Quantifiers
$\neg \forall x P(x) \equiv \exists x \neg P (x)$
example
$\neg (\forall x (x > 3)) \equiv \exists x \neg (x > 3) \equiv \exists x (x \leq 3)$

in a sequence of quantifiers, apply de morgans law from outside to inside
example
$\neg \forall x \forall y P(x,y)$
$\equiv \exists x \neg(\forall y P(x,y))$
$\equiv \exists x \exists y \neg P (x, y)$


