tags: #notes #fleeting
creation date: [[2022-11-09 Wednesday]] 11:01:40
description:: recursively defined functions and sets

## Recursive definitions
- Recursively defined functions:
	- We use two steps to define a function $f : N \rightarrow N$:
	- **Basis step**:
		- Specify the value of the function at some starting point
		- e.g., at 0 or 1, or at some $b$
	- **Recursive step**:
		- Give a rule for finding its value at an integer from its value at smaller integers.

- ex. $F(0) = 1$ and $F(n) = nF(n-1)$ for $n \geq 1$
	- $= n!$
- ex. $f_0 = 0, f_1 = 1$, and $f_n = f_{n-1} + f_{n-2}$ for $n \geq 2$
	- fibonacci sequence
	- 0 1 1 2 3 5 8 ...
- ex. $T(1) = 1$ and $T(n) = 1 + T(\lfloor \frac n 2 \rfloor)$ for $n \geq 2$
	- time for binary search
- ex. $T(1) = 1$ and $T(n) = 2T(\lfloor \frac n 2 \rfloor) + n$ for $n \geq 2$
	- time for fast sorting
- ex. $f(0) = 1$, $f(n) = f(n-1) + r^n$, $n \geq 1$
	- sum of the $n+1$ terms of the geometric series
- ex. $f(2) = 1$, $f(n) = 1 + f(\log n), \forall n > 2$
	- what is this function?
	- If $n = 2^k$, $f(n) = 1 + f(\log 2^k ) = 1+ f(k)$. Similarly $f(2^{2^k}) = 1 + f(2^k) = 2+ f(k)$. E.g., $f(2^{16}) = 1 + f(16) = 1+1+ f(4) = 1+1+1+ f(2) = 4$. Then $f(2^{2^16}) = 5$. So $f = \log ^âˆ—$
	- i.e., the number of times we must apply log to get to 1
	- For non-powers of 2 it needs broader definition: 
	  $f(n) = 1$, if $0 < n \leq 2$ 
	  $f(n) = 1 + f(\log n)$ for $n > 2$
	- um ok

- Recursively defined sets:
	- ex.
		- Basis: $2 \in S$
		- Recursive step: if $x, y \in S$, then $x + y \in S$ 
		- the set contains all positive even numbers
	- ex.
		- The set $\sum^*$ of all strings over the alphabet $\sum$ can be defined as:
		- Basis step: Empty string $\epsilon \in \sum ^*$ (i.e., $\epsilon = \emptyset$)
		- Recursive step: For any $w \in \sum ^*$ and $a \in \sum$, $wa \in \sum^*$
		- e.g., $\sum = \{0,1\}$. $\sum ^* = \{\emptyset, \{0\}, \{1\}, \{00\}, \{01\}, \{10\}, \{11\}, \{000\}, \ldots \}$
		- A related function is the length of a string, defined recursively similarly to the above: $l(\epsilon) = 0$ and $l(wx) = l(w) + 1, \forall w \sum^*$, $x \in \sum$
		- 