tags: #notes #fleeting
creation date: [[2022-09-12 Monday]] 10:54:46
description:: quantifiers, rules of inference, tautology

new classroom
wren 301 (jesus man you couldve sent an email)

hw #1 due on wednesday
- [x] i should do hw #1 cs243 today or tmr
some questions include quantifiers and mix of quantifiers

## Quantifiers cont.
##### Quantifier Example
$\forall x \exists y (x+y = 0)$
for all x, there exists a y such that ...
this is a proposition (and a true one, if x = 5, y = -5, etc)
how do we prove this for all cases?
"if youre trying to prove something is false, is one example sufficient" "well, yes, ... well get to that"

##### Answer
$\forall x \exists y (x+y = 0)$
true because for any x, y can be -x

for any positive integer x is it true there exists a positive integer y to satisfy? no y has to be negative here
know the domains of the problems
"depends on what universe we're looking for"

##### Order matters
$\exists y \forall x (x + y = 0)$
there exists a y such that for all x, x + y = 0
impossible
here is where a counter example would prove this is false
ex.
y = 5
for any x, we pick 3
5 + 3 does not equal 0, so false

$\exists y \forall x (x + y = 0)$
false because pick any $y_0$
any x does not equal $-y_0$
the equation doesnt hold

##### Order doesnt matter
$\forall x \forall y \forall z P(x, y, z)$
if all quantifiers are the same then order doesnt matter


in class question
$\exists x \forall y (x * y = 0)$
an example of a "there exists" and then a "for all" that is true
doesnt have to be $\forall$ and then $\exists$

^ this was all review i guess for the hw and wrapping up quantifiers from last class

## Rules of Inference

##### Argument
different from a proposition
google "the argument" monty python skit
and then forget it our argument is not like that argument

Argument - a sequence of statements that ends in a conclusion
ex. my shoes are shiny, the sun is bright, therefore i need to eat lunch

Valid argument - if premises (preceding statements) are true, then the conclusion (final statement) must be true

have to find logical ways to go from statement to statement

Argument:
- prop 1
- prop 2
- ...
- prop x
- $\downarrow$
- conclusion

Inference - getting from statement to statement
"remember this"

##### Modus Ponens
$p$
$p \rightarrow q$
=
$q$

"the basis" "without modus ponens there is no logic"
"just remember this ones name"

##### Modus Tollens
$\neg q$
$p \rightarrow q$
=
$\neg p$

the negative of modus ponens basically

##### Hypothetical Syllogism
$p \rightarrow q$
$q \rightarrow r$
=
$p \rightarrow r$

"all ferraris are red"
"all red cars get tickets"
so
"all ferraris get tickets"

##### Disjunctive Syllogism
$p \bigvee q$
$\neg p$
=
$q$


##### Addition
$p$
$p \bigvee q$
=
$q$

"uhh think the notes are wrong"

##### Simplification
$p \bigwedge q$
$=$
$p$

i am old and rich
so
i am old

##### Conjunction
$p$
$q$
=
$p \bigwedge q$


##### Resolution
$p \bigvee q$
$\neg p \bigvee r$
=
$q \bigvee r$

my car is a ferrari or an audi
my car is not a ferrari or it is red
so
my car is an audi or it is red

"when you are combining these statements you are $\bigwedge$ing them"
$(p \bigvee q) \bigwedge (\neg p \bigvee r) \equiv q \bigvee r$
same as this
distribution
"not an obvious proof"

i read a book or went to the movies
i did not read a book or i went for dinner
so
i went to the movies or i went for dinner


these laws are powerful for automatic theorem proving
"might spend a few classes on automatic theorem proving tools"


## Tautology
a propositional function which is always True
ex. x = x
ex. T 
- "Truth itself is a tautology"
ex. $(p \bigvee q) \bigwedge (\neg p \bigvee r) \equiv q \bigvee r$ 
- resolution proposition from earlier
- is always true, can prove

lets prove modus ponens; can be represented as $(p \bigwedge (p \rightarrow q)) \rightarrow q$
first drop implications
remember cereal box $a \rightarrow b \equiv \neg a \bigvee b$
can start with either, inside or outside
$\equiv (p \bigwedge ( \neg p \bigvee q )) \rightarrow q)$
distribute p:
$\equiv ( (p \bigwedge \neg p) \bigvee (p \bigwedge q) ) \rightarrow q$
p and not p cannot be true, it is false:
$\equiv (F \bigvee (p \bigwedge q) \rightarrow q$
using identity rule
$\equiv (p \bigwedge q) \rightarrow q$
apply our cereal box formula again to get rid of implication
$\equiv \neg(p\bigwedge q) \bigvee q$
de morgan
$\equiv \neg p \bigvee \neg q \bigvee q$
$\equiv \neg p \bigvee T$
$\equiv T$
