tags: #notes #fleeting
creation date: [[2022-09-16 Friday]] 11:03:57
description:: methods of proof

#### Proof by Contraposition
if p then q
assume q is false and prove p is false
$p \rightarrow q \equiv \neg q \rightarrow \neg p$

ex. Prove that if $n = a*b$, where $a , b$ are positive integers,
then $a \leq \sqrt {n}$ or $b \leq \sqrt {n}$

p = n = ab $\wedge$ a pos int $\wedge$ b pos int
q = $a \leq \sqrt {n} \vee b \leq \sqrt {n}$

$\neg q = \neg (a \leq \sqrt {n} \vee b \leq \sqrt {n})$
$= a \gt \sqrt {n} \wedge b \gt \sqrt {n}$

then n = $a*b \gt \sqrt n * \sqrt n$
= $a*b \gt n$
$a*b \neq n$

we proved that $\neg q \rightarrow \neg p$
therefore, $p \rightarrow q$


##### Contradiction
given proposition
want to prove p
"more general in a way"

to prove p, assume p is false
and show there is a proposition $r$ such that *r* is true *and* $\neg r$ is true, therefore $(r \wedge \neg r)$, which is a contradiction

$p \equiv \neg p \rightarrow (r \wedge \neg r)$

OR, according to textbook, assume both $p$ is true and $\neg q$ is true
then you can show $p \wedge \neg p$
or you can show $q \wedge \neg q$
to prove by contradiction

ex. prove that $\sqrt 2$ is an irrational number
Assume $\sqrt 2$ is not irrational, ie $\sqrt 2$ rational.
By def of rational numbers, $\exists a, b$ integers with gcd(a,b) = 1 such that $\sqrt 2 = \frac a b$

square both sides:  $2 = \frac {a^2} {b^2}$
$=> 2b^2 = a^2$
$a^2$ must be even
so $a$ is even also
	proof:
	if a were odd, then $a*a$ would also be odd
	$a^2$ odd $\wedge a^2$ even
	contradiction
by def. of even numbers, there exists some integer c
$\exists c (a = 2c)$
then $2b^2 = a^2 = (2c)^2 = 4c^2$
$b^2 = 2c^2$
therefore b is even too

gcd(a,b) = 2 $\wedge$ gcd(a,b) = 1
contradiction

difference between contraposition and contradiction is subtle
in doing proofs, people usually dont distinguish between the two, just call both "proof by contradiction"
	contraposition shows $p \rightarrow q$
	contradiction shows $p$
to use contradiction to show $p \rightarrow q$, assume $\neg (p \rightarrow q) = p \wedge \neg q$ (got here using cereal box equivalences) and show $\neg p$.
then, we have $p \wedge \neg p$ which is a contradiction


##### Proof by Cases
When we are unable to prove a theorem with a single argument that hold for all possible cases, we may need to construct our proof for each of the possible cases, one by one.
The rule of inference behind this method lies on
$(p_1 \vee p_2 \vee ... \vee p_n) \rightarrow q$
$\equiv (p_1 \rightarrow q) \wedge (p_2 \rightarrow q) \wedge ... \wedge (p_n \rightarrow q)$

